First implementation of `Derive`

code/SAT.v
@@ -8,11 +8,16 @@ Inductive Literal : Type :=
     | posLit (p: Atom)
     | negLit (p: Atom).
 
+Notation "+ p" := (posLit p) (at level 35, right associativity).
+Notation "- p" := (negLit p) (at level 35, right associativity).
+
 Definition negateLiteral (l: Literal) : Literal :=
     match l with
-    | posLit p => negLit p
-    | negLit p => posLit p
+    | +p => -p
+    | -p => +p
     end.
+
+Notation "~ l" := (negateLiteral l) (at level 75, right associativity).
 
 (* A clause is a disjunction of literals. *)
 Definition Clause := list Literal.
@@ -20,43 +25,86 @@ Definition Clause := list Literal.
 (* A formula is a conjunction of clauses. *)
 Definition Formula := list Clause.
 
+(* The antecedent is the reason for the value of a set literal. *)
+Inductive Antecedent : Type :=
+    | decided
+    | propagated.
+
 Definition negateClause (c: Clause) : Formula :=
-    map (fun (l: Literal) => [negateLiteral l]) c.
+    map (fun (l: Literal) => [~l]) c.
 
-(* A partial assignment for atoms to true or false.
-   Note that `d` indicates if the assignment was a decision. *)
+(* A partial assignment for atoms to true or false. *)
 Inductive PartialAssignment : Type :=
-  | empty
-  | record (p: Atom) (v d: bool) (m: PartialAssignment).
+    | empty
+    | record (p: Atom) (v: bool) (a: Antecedent) (m: PartialAssignment).
 
-Definition setAtom (m: PartialAssignment) (p: Atom) (v d: bool) : PartialAssignment :=
-    record p v d m.
+Fixpoint appendPartialAssignment (m n: PartialAssignment) : PartialAssignment :=
+    match n with
+    | empty => m
+    | record p' v' a' n' =>  record p' v' a' (appendPartialAssignment m n')
+    end.
 
-Definition setLiteral (m: PartialAssignment) (l: Literal) (d: bool) : PartialAssignment :=
+Notation "m ++a n" := (appendPartialAssignment m n) (at level 65, left associativity).
+
+Definition setAtom (m: PartialAssignment) (p: Atom) (v: bool) (a: Antecedent): PartialAssignment :=
+    record p v a m.
+
+Definition setLiteral (m: PartialAssignment) (l: Literal) (a: Antecedent) : PartialAssignment :=
     match l with
-    | posLit p => setAtom m p true d
-    | negLit p => setAtom m p false d
+    | +p => setAtom m p true a
+    | -p => setAtom m p false a
+    end.
+
+Definition decideLiteral (m: PartialAssignment) (l: Literal) : PartialAssignment :=
+    setLiteral m l decided.
+
+Notation "m ++d l" := (decideLiteral m l) (at level 65, left associativity).
+
+Definition propagateLiteral (m: PartialAssignment) (l: Literal) : PartialAssignment :=
+    setLiteral m l propagated.
+
+Notation "m ++p l" := (propagateLiteral m l) (at level 65, left associativity).
+
+Fixpoint antecedentAtom (m: PartialAssignment) (p: Atom) : option Antecedent :=
+    match m with
+    | empty => None
+    | record p' v' a' m' => if p =? p' then Some a' else antecedentAtom m' p'
+    end.
+
+Definition antecedentLiteral (m: PartialAssignment) (l: Literal) : option Antecedent :=
+    match l with
+    | +p => antecedentAtom m p
+    | -p => antecedentAtom m p
     end.
 
 Fixpoint evalAtom (m: PartialAssignment) (p: Atom) : option bool :=
     match m with
     | empty => None
-    | record p' v' d' m' => if p =? p' then Some v' else evalAtom m' p'
+    | record p' v' a' m' => if p =? p' then Some v' else evalAtom m' p
     end.
 
 Definition evalLiteral (m: PartialAssignment) (l: Literal) : option bool :=
     match l with
-    | posLit p => evalAtom m p
-    | negLit p => option_map negb (evalAtom m p)
+    | +p => evalAtom m p
+    | -p => option_map negb (evalAtom m p)
     end.
 
 (* An atom is defined if it is assigned true or false. *)
 Definition DefinedAtom (m: PartialAssignment) (p: Atom) : Prop :=
     exists (v: bool), evalAtom m p = Some v.
 
+Definition UndefinedAtom (m: PartialAssignment) (p: Atom) : Prop :=
+    ~DefinedAtom m p.
+
 (* A literal is defined if its atom is assigned true or false. *)
 Definition DefinedLiteral (m: PartialAssignment) (l: Literal) : Prop :=
     exists (v: bool), evalLiteral m l = Some v.
+
+Definition UndefinedLiteral (m: PartialAssignment) (l: Literal) : Prop :=
+    ~DefinedLiteral m l.
+
+Definition NoDecisionLiterals (m: PartialAssignment) : Prop :=
+  forall (l: Literal), DefinedLiteral m l -> antecedentLiteral m l = Some propagated.
 
 (* A partial assignment is total if all atoms are assigned true or false.
    The number of atoms is given by `n`. *)
@@ -101,9 +149,9 @@ Fixpoint evalFormula (m: PartialAssignment) (f: Formula) : option bool :=
         end
     end.
 
-Compute evalFormula (record 5 true true empty) [[negLit 5]].
-Compute evalFormula (record 5 true true empty) [[posLit 5]].
-Compute evalFormula (record 5 true true empty) [[postLit 6]].
+Compute evalFormula (empty ++d +5) [[-(5)]]. (* Some false *)
+Compute evalFormula (empty ++d +5) [[+5]].   (* Some true *)
+Compute evalFormula (empty ++d +5) [[+6]].   (* None *)
 
 Definition Model (m: PartialAssignment) (f: Formula) : Prop :=
     evalFormula m f = Some true.
@@ -121,16 +169,135 @@ Definition Equivalent (f f': Formula) : Prop :=
     Entails f f' /\ Entails f' f.
 
 Inductive State : Type :=
-    | fail
-    | state (m: PartialAssignment) (f: Formula).
+    | failState (depth: nat)
+    | state (depth: nat) (m: PartialAssignment) (f: Formula).
 
 Fixpoint toFormula (m: PartialAssignment) : Formula :=
     match m with
     | empty => []
     | record p' v' d' m' =>
-        if v' then [posLit p'] :: (toFormula m')
-        else [negLit p'] :: (toFormula m')
+        if v' then (toFormula m') ++ [[+p']]
+        else (toFormula m') ++ [[-p']]
     end.
 
 Definition Conflicting (m: PartialAssignment) (c: Clause) : Prop :=
     Entails (toFormula m) (negateClause c).
+
+Inductive Derived : State -> Prop :=
+    (* If a clause is false except for one unassigned literal, assign it to satisfy the clause. *)
+    | unitPropagate (d: nat) (m: PartialAssignment) (f: Formula) (l: Literal) (c: Clause) :
+        (* The literal is in the clause. *)
+        In l c ->
+        (* The clause is in the formula. *)
+        In c f ->
+        (* There is at least one non-false literal in the clause.  *)
+        evalClause m c = None ->
+        (* The literal must be an unassigned literal. *)
+        evalClause (m ++d ~l) c = Some false ->
+        Derived (state d m f) ->
+        Derived (state (S d) (m ++p l) f)
+
+    (* If a literal appears only positively in f, it must be true. *)
+    | pureLiteral (d: nat) (m: PartialAssignment) (f: Formula) (l: Literal) (c: Clause) :
+        (* The literal is in the clause. *)
+        In l c ->
+        (* The clause is in the formula. *)
+        In c f ->
+        (* The literal is not defined yet. *)
+        UndefinedLiteral m l ->
+        (* The negation of the literal appears nowhere in no clause of the formula. *)
+        ~(exists (c': Clause), In (~l) c' /\ In c' f) ->
+        Derived (state d m f) ->
+        Derived (state (S d) (m ++p l) f)
+
+    (* Arbitrarily set an unassigned literal to true. *)
+    | decide (d: nat) (m: PartialAssignment) (f: Formula) (l: Literal) (c: Clause) :
+        (* The literal is in the clause. *)
+        In l c ->
+        (* The clause is in the formula. *)
+        In c f ->
+        (* The literal is not defined yet. *)
+        UndefinedLiteral m l ->
+        Derived (state d m f) ->
+        Derived (state (S d) (m ++d l) f)
+
+    (* Fail if all literals are assigned and there is a conflict. *)
+    | fail (d: nat) (m: PartialAssignment) (f: Formula) (c: Clause) :
+        (* The clause is in the formula. *)
+        In c f ->
+        (* The partial assignment is conflicting with the clause. *)
+        Conflicting m c ->
+        (* There are no decision literals to backtrack to. *)
+        NoDecisionLiterals m ->
+        Derived (state d m f) ->
+        Derived (failState (S d))
+
+    (* Backtrack by flipping the most recent decision literal. *)
+    | backtrack (d: nat) (m n: PartialAssignment) (f: Formula) (l: Literal) (c: Clause) :
+        let mln := m ++d l ++a n in
+        (* The clause is in the formula. *)
+        In c f ->
+        (* The partial assignment is conflicting with the clause. *)
+        Conflicting mln c ->
+        (* There are no decision literals to backtrack to in n. *)
+        NoDecisionLiterals n ->
+        (* The literal l is the most recent decision literal to backtrack to. *)
+        antecedentLiteral mln l = Some decided ->
+        Derived (state d mln f) ->
+        Derived (state (S d) (m ++d ~l) f).
+
+Definition singleClause : Formula := [[+1; +2; +3]].
+Definition firstTwoFalse : PartialAssignment := empty ++d -(1) ++d -(2).
+Example unitPropagationSingleClause :
+    Derived (state 0 firstTwoFalse singleClause) ->
+    Derived (state 1 (firstTwoFalse ++p +3) singleClause).
+Proof.
+    apply unitPropagate with [+1; +2; +3].
+    - simpl. right. right. left. reflexivity.
+    - simpl. left. reflexivity.
+    - simpl. reflexivity.
+    - simpl. reflexivity.
+Qed.
+
+Definition twoClauses : Formula := [[+1; +2];[+1; +3]].
+Example pureLiteralTwoClauses :
+    Derived (state 0 empty twoClauses) ->
+    Derived (state 1 (empty ++p +1) twoClauses).
+Proof.
+    apply pureLiteral with [+1; +2].
+    - simpl. left. reflexivity.
+    - simpl. left. reflexivity.
+    - unfold UndefinedLiteral. unfold DefinedLiteral, not. simpl. intros. destruct H as [v H]. discriminate H.
+    - unfold not. simpl. intros. destruct H as [c [H [G1|[G2|G3]]]].
+        * rewrite <- G1 in H. simpl in H. destruct H as [H1|[H2|H3]].
+            + discriminate.
+            + discriminate.
+            + contradiction.
+        * rewrite <- G2 in H. simpl in H. destruct H as [H1|[H2|H3]].
+            + discriminate.
+            + discriminate.
+            + contradiction.
+        * contradiction.
+Qed.
+
+Example decideSingleClause :
+    Derived (state 0 empty singleClause) ->
+    Derived (state 1 (empty ++d +1) singleClause).
+Proof.
+    apply decide with [+1; +2; +3].
+    - simpl. left. reflexivity.
+    - simpl. left. reflexivity.
+    - unfold UndefinedLiteral. unfold DefinedLiteral, not. simpl. intros. destruct H as [v H]. discriminate.
+Qed.
+
+Definition allThreeFalse : PartialAssignment := firstTwoFalse ++d -(3).
+Example backtrackSingleClause :
+    Derived (state 0 allThreeFalse singleClause) ->
+    Derived (state 1 (firstTwoFalse ++d +3) singleClause).
+Proof.
+    apply backtrack with (m := firstTwoFalse) (l := -(3)) (n := empty) (c := [+1; +2; +3]).
+    - simpl. left. reflexivity.
+    - unfold Conflicting. unfold Entails. simpl. intros. assumption.
+    - unfold NoDecisionLiterals. unfold DefinedLiteral. intros. destruct H as [v H]. destruct l; simpl in H; discriminate.
+    - simpl. reflexivity.
+Qed.
